fstar/symbolic/MLS.Symbolic.MyMkRand.fst
@@ -1,0 +1,88 @@
+module MLS.Symbolic.MyMkRand
+
+open DY.Core
+
+#set-options "--fuel 0 --ifuel 0"
+
+[@@ "opaque_to_smt"]
+val my_mk_rand: usg:usage -> lab:(bytes -> label) -> len:nat{len <> 0} -> traceful bytes
+let my_mk_rand usg lab len =
+  let* time = get_time in
+  let result = (Rand len time) in
+  add_event (RandGen usg (lab result) len);*
+  return result
+
+/// Generating a random bytestrings always preserve the trace invariant.
+
+#push-options "--z3rlimit 25 --fuel 1 --ifuel 1"
+val my_mk_rand_trace_invariant:
+  {|protocol_invariants|} ->
+  usg:usage -> lab:(bytes -> label) -> len:nat{len <> 0} -> tr:trace ->
+  Lemma
+  (requires trace_invariant tr)
+  (ensures (
+    let (b, tr_out) = my_mk_rand usg lab len tr in
+    trace_invariant tr_out /\
+    1 <= DY.Core.Trace.Base.length tr_out /\
+    rand_generated_at tr_out (DY.Core.Trace.Base.length tr_out - 1) b
+  ))
+  [SMTPat (my_mk_rand usg lab len tr); SMTPat (trace_invariant tr)]
+let my_mk_rand_trace_invariant #invs usg lab len tr =
+  let result = (Rand len (DY.Core.Trace.Base.length tr)) in
+  add_event_invariant (RandGen usg (lab result) len) tr;
+  reveal_opaque (`%my_mk_rand) (my_mk_rand)
+#pop-options
+
+/// Random bytestrings satisfy the bytes invariant.
+
+#push-options "--fuel 1 --ifuel 1"
+val my_mk_rand_bytes_invariant:
+  {|protocol_invariants|} ->
+  usg:usage -> lab:(bytes -> label) -> len:nat{len <> 0} -> tr:trace ->
+  Lemma
+  (ensures (
+    let (b, tr_out) = my_mk_rand usg lab len tr in
+    bytes_invariant tr_out b
+  ))
+  // We need a way for the SMT pattern to know the value of `invs`
+  // This is done using `trace_invariant`, although it is not necessary for the theorem to hold,
+  // it is certainly around in the context
+  [SMTPat (my_mk_rand usg lab len tr); SMTPat (trace_invariant tr)]
+let my_mk_rand_bytes_invariant #invs usg lab len tr =
+  reveal_opaque (`%my_mk_rand) (my_mk_rand);
+  normalize_term_spec bytes_invariant
+#pop-options
+
+/// Label of random bytestrings.
+
+#push-options "--fuel 1 --ifuel 1"
+val my_mk_rand_get_label:
+  {|protocol_invariants|} ->
+  usg:usage -> lab:(bytes -> label) -> len:nat{len <> 0} -> tr:trace ->
+  Lemma
+  (ensures (
+    let (b, tr_out) = my_mk_rand usg lab len tr in
+    get_label tr_out b == lab b
+  ))
+  [SMTPat (my_mk_rand usg lab len tr); SMTPat (trace_invariant tr)]
+let my_mk_rand_get_label #invs usg lab len tr =
+  reveal_opaque (`%my_mk_rand) (my_mk_rand);
+  normalize_term_spec get_label
+#pop-options
+
+/// Usage of random bytestrings.
+
+#push-options "--fuel 1 --ifuel 1"
+val my_mk_rand_has_usage:
+  {|protocol_invariants|} ->
+  usg:usage -> lab:(bytes -> label) -> len:nat{len <> 0} -> tr:trace ->
+  Lemma
+  (ensures (
+    let (b, tr_out) = my_mk_rand usg lab len tr in
+    b `has_usage tr_out` usg
+  ))
+  [SMTPat (my_mk_rand usg lab len tr); SMTPat (trace_invariant tr)]
+let my_mk_rand_has_usage #invs usg lab len tr =
+  normalize_term_spec my_mk_rand;
+  normalize_term_spec has_usage
+#pop-options
