fstar/treesync/symbolic/MLS.TreeSync.Symbolic.SignatureKeyState.fst
@@ -1,0 +1,167 @@
+module MLS.TreeSync.Symbolic.SignatureKeyState
+
+open Comparse
+open DY.Core
+open DY.Lib
+open MLS.Symbolic
+open MLS.Symbolic.MyMkRand
+
+#set-options "--fuel 0 --ifuel 0"
+
+[@@ with_bytes bytes]
+type treesync_signature_key_state = {
+  signature_sk: bytes;
+}
+
+%splice [ps_treesync_signature_key_state] (gen_parser (`treesync_signature_key_state))
+%splice [ps_treesync_signature_key_state_is_well_formed] (gen_is_well_formed_lemma (`treesync_signature_key_state))
+
+instance local_state_treesync_signature_key_state: local_state treesync_signature_key_state = {
+  tag = "MLS.TreeSync.SignatureKeyState";
+  format = mk_parseable_serializeable ps_treesync_signature_key_state;
+}
+
+val signature_key_label_pred:
+  principal -> bytes ->
+  principal -> string -> state_id -> treesync_signature_key_state -> prop
+let signature_key_label_pred prin1 signature_vk =
+  fun prin2 tag sid st ->
+    prin1 == prin2 /\
+    tag == "MLS.TreeSync.SignatureKeyState" /\
+    vk st.signature_sk == signature_vk
+
+val signature_key_label:
+  principal -> bytes ->
+  label
+let signature_key_label prin signature_vk =
+  typed_state_pred_label (signature_key_label_pred prin signature_vk)
+
+val signature_key_label_can_flow_public:
+  tr:trace ->
+  prin:principal -> signature_vk:bytes ->
+  Lemma
+  (requires
+    (signature_key_label prin signature_vk) `can_flow tr` public
+  )
+  (ensures
+    exists sid signature_sk.
+      state_was_corrupt tr prin "MLS.TreeSync.SignatureKeyState" sid { signature_sk } /\
+      vk signature_sk == signature_vk
+  )
+let signature_key_label_can_flow_public tr prin signature_vk = ()
+
+val is_signature_key_sk: {|crypto_invariants|} -> trace -> principal -> bytes -> prop
+let is_signature_key_sk #cinvs tr prin signature_sk =
+  bytes_invariant tr signature_sk /\
+  get_label tr signature_sk == signature_key_label prin (vk signature_sk) /\
+  signature_sk `has_usage tr` mk_mls_sigkey_usage prin
+
+val is_signature_key_vk: {|crypto_invariants|} -> trace -> principal -> bytes -> prop
+let is_signature_key_vk #cinvs tr prin signature_vk =
+  bytes_invariant tr signature_vk /\
+  get_signkey_label tr signature_vk == signature_key_label prin signature_vk /\
+  signature_vk `has_signkey_usage tr` mk_mls_sigkey_usage prin
+
+val treesync_signature_key_state_pred: {|crypto_invariants|} -> local_state_predicate treesync_signature_key_state
+let treesync_signature_key_state_pred #cinvs = {
+  pred = (fun tr prin sid content ->
+    is_signature_key_sk tr prin content.signature_sk
+  );
+  pred_later = (fun tr1 tr2 prin sid content -> ());
+  pred_knowable = (fun tr prin sid content -> ());
+}
+
+val has_treesync_signature_key_state_invariant: {|protocol_invariants|} -> prop
+let has_treesync_signature_key_state_invariant #invs =
+  has_local_state_predicate treesync_signature_key_state_pred
+
+val treesync_signature_key_state_tag_and_invariant: {|crypto_invariants|} -> dtuple2 string local_bytes_state_predicate
+let treesync_signature_key_state_tag_and_invariant #ci = (|local_state_treesync_signature_key_state.tag, local_state_predicate_to_local_bytes_state_predicate treesync_signature_key_state_pred|)
+
+val signature_sk_to_signature_key_label:
+  principal -> bytes ->
+  label
+let signature_sk_to_signature_key_label prin signature_sk =
+  signature_key_label prin (vk signature_sk)
+
+val mk_signature_key:
+  principal ->
+  traceful state_id
+let mk_signature_key prin =
+  let* sk = my_mk_rand (mk_mls_sigkey_usage prin) (signature_sk_to_signature_key_label prin) 32 in
+  let* sid = new_session_id prin in
+  set_state prin sid { signature_sk = sk; };*
+  return sid
+
+val mk_signature_key_invariant:
+  {|protocol_invariants|} ->
+  prin:principal ->
+  tr:trace ->
+  Lemma
+  (requires
+    trace_invariant tr /\
+    has_treesync_signature_key_state_invariant
+  )
+  (ensures (
+    let (sid, tr_out) = mk_signature_key prin tr in
+    trace_invariant tr_out
+  ))
+  [SMTPat (mk_signature_key prin tr);
+   SMTPat (trace_invariant tr)]
+let mk_signature_key_invariant #invs prin tr = ()
+
+val get_signature_key_sk:
+  principal -> state_id ->
+  traceful (option bytes)
+let get_signature_key_sk prin sid =
+  let*? st = get_state prin sid in
+  return (Some (st.signature_sk))
+
+val get_signature_key_sk_invariant:
+  {|protocol_invariants|} ->
+  prin:principal -> sid:state_id ->
+  tr:trace ->
+  Lemma
+  (requires
+    trace_invariant tr /\
+    has_treesync_signature_key_state_invariant
+  )
+  (ensures (
+    let (opt_signature_sk, tr_out) = get_signature_key_sk prin sid tr in
+    tr_out == tr /\ (
+      match opt_signature_sk with
+      | None -> True
+      | Some signature_sk -> is_signature_key_sk tr prin signature_sk
+    )
+  ))
+  [SMTPat (get_signature_key_sk prin sid tr);
+   SMTPat (trace_invariant tr)]
+let get_signature_key_sk_invariant #invs prin sid tr = ()
+
+val get_signature_key_vk:
+  principal -> state_id ->
+  traceful (option bytes)
+let get_signature_key_vk prin sid =
+  let*? sk = get_signature_key_sk prin sid in
+  return (Some (vk sk))
+
+val get_signature_key_vk_invariant:
+  {|protocol_invariants|} ->
+  prin:principal -> sid:state_id ->
+  tr:trace ->
+  Lemma
+  (requires
+    trace_invariant tr /\
+    has_treesync_signature_key_state_invariant
+  )
+  (ensures (
+    let (opt_signature_vk, tr_out) = get_signature_key_vk prin sid tr in
+    tr_out == tr /\ (
+      match opt_signature_vk with
+      | None -> True
+      | Some signature_vk -> is_signature_key_vk tr prin signature_vk
+    )
+  ))
+  [SMTPat (get_signature_key_vk prin sid tr);
+   SMTPat (trace_invariant tr)]
+let get_signature_key_vk_invariant #invs prin sid tr = ()
